Tealeaves/Examples/VariadicLet/Demo.v
@@ -11,99 +11,64 @@ Variables (x y z : atom).
 Definition term1: term LN :=
   letin [tvar (Fr x)] (tvar (Bd 0)).
 Definition term2: term LN :=
-  letin [tvar (Bd 0)] (tvar (Fr y)).
+  letin [tvar (Bd 0)] (tvar (Bd 0)).
 Definition term3: term LN :=
-  letin [tvar (Fr x); tvar (Bd 0)] (tvar (Fr y)).
-Definition term3a: term LN :=
-    letin [tvar (Fr x); tvar (Bd 0); tvar (Bd 1)] (tvar (Fr y)).
+  letin [tvar (Fr x); tvar (Bd 1)] (tvar (Bd 1)).
 Definition term4: term LN :=
-  letin [tvar (Bd 1) ; tvar (Bd 0)] (tvar (Fr y)).
+  letin [tvar (Bd 0); tvar (Bd 1) ; tvar (Bd 2)] (tvar (Bd 2)).
+Definition term5: term LN :=
+  letin [tvar (Bd 1) ; tvar (Bd 2) ; tvar (Bd 3)] (tvar (Bd 2)).
 
 Module demo1.
 
   Import Simple.
 
-  Notation "'LC'" :=
-    (LCnb
-       (Mapdt_U_inst:=Mapdt_term)) (at level 10).
-  Notation "'GAP'" :=
-    (local_closure_gap
-       (Mapdt_U_inst:=Mapdt_term)) (at level 10).
+  Goal LCnb 0 term1 = true. reflexivity. Qed.
 
-  Goal LC 0 term1 = true. reflexivity. Qed.
+  Goal LCnb 0 term2 = false. reflexivity. Qed.
+  Goal LCnb 1 term2 = true. reflexivity. Qed.
 
-  Goal LC 0 term2 = false. reflexivity. Qed.
-  Goal LC 1 term2 = true. reflexivity. Qed.
+  Goal LCnb 0 term3 = false. reflexivity. Qed.
+  Goal LCnb 1 term3 = false. reflexivity. Qed.
 
-  Goal LC 0 term3 = false. reflexivity. Qed.
-  Goal LC 1 term3 = true. reflexivity. Qed.
-  Goal LC 1 term3a = false. reflexivity. Qed.
+  Goal LCnb 0 term5 = false. reflexivity. Qed.
+  Goal LCnb 1 term5 = false. reflexivity. Qed.
+  Goal LCnb 2 term5 = false. reflexivity. Qed.
 
-  Goal LC 0 term4 = false. reflexivity. Qed.
-  Goal LC 1 term4 = false. reflexivity. Qed.
-  Goal LC 2 term4 = true. reflexivity. Qed.
-
-  Example ex1: GAP term1 = 0 := ltac:(trivial).
-  Example ex2: GAP term2 = 1 := ltac:(trivial).
-  Example ex3: GAP term3 = 1 := ltac:(trivial).
-  Example ex3a: GAP term3a = 2 := ltac:(trivial).
-  Example ex4: GAP term4 = 2 := ltac:(trivial).
+  Example ex1: level term1 = 0 := ltac:(trivial).
+  Example ex2: level term2 = 1 := ltac:(trivial).
+  Example ex3: level term3 = 2 := ltac:(trivial).
+  Example ex4: level term4 = 3 := ltac:(trivial).
+  Example ex5: level term5 = 4 := ltac:(trivial).
 
 End demo1.
 
 Module demo2.
 
-  Import ex_binding_type2.
+  Import LetIn.
 
-  Notation "'LC'" :=
-    (locally_closed_gap_bool
-       (Mapdt_U_inst:=Mapdt_term)) (at level 10).
-  Notation "'GAP'" :=
-    (local_closure_gap
-       (Mapdt_U_inst:=Mapdt_term)) (at level 10).
-
-  Goal LC 0 term1 = true. reflexivity. Qed.
-
-  Goal LC 0 term2 = false. reflexivity. Qed.
-  Goal LC 1 term2 = true. reflexivity. Qed.
-
-  Goal LC 0 term3 = true. reflexivity. Qed.
-  Goal LC 0 term3a = true. reflexivity. Qed.
-
-  Goal LC 0 term4 = false. reflexivity. Qed.
-  Goal LC 1 term4 = false. reflexivity. Qed.
-  Goal LC 2 term4 = true. reflexivity. Qed.
-
-  Example ex1: GAP term1 = 0 := ltac:(trivial).
-  Example ex2: GAP term2 = 1 := ltac:(trivial).
-  Example ex3: GAP term3 = 0 := ltac:(trivial).
-  Example ex3a: GAP term3a = 0 := ltac:(trivial).
-  Example ex4: GAP term4 = 2 := ltac:(trivial).
+  Example ex1: level term1 = 0 := ltac:(trivial).
+  Example ex2: level term2 = 1 := ltac:(trivial).
+  Example ex3: level term3 = 1 := ltac:(trivial).
+  Example ex4: level term4 = 1 := ltac:(trivial).
+  Example ex5: level term5 = 2 := ltac:(trivial).
 
 End demo2.
 
 Module demo3.
 
-  Import ex_binding_type3.
-  Notation "'LC'" :=
-    (locally_closed_gap_bool
-       (Mapdt_U_inst:=Mapdt_term)) (at level 10).
-  Notation "'GAP'" :=
-    (local_closure_gap
-       (Mapdt_U_inst:=Mapdt_term)) (at level 10).
+  Import LetRec.
 
-  Goal LC 0 term1 = true. reflexivity. Qed.
+  Goal LCnb 0 term1 = true. reflexivity. Qed.
 
-  Goal LC 0 term2 = true. reflexivity. Qed.
+  Goal LCnb 0 term2 = true. reflexivity. Qed.
 
-  Goal LC 0 term3 = true. reflexivity. Qed.
+  Goal LCnb 0 term3 = true. reflexivity. Qed.
 
-  Goal LC 0 term4 = true. reflexivity. Qed.
 
-  Example ex1: GAP term1 = 0 := ltac:(trivial).
-  Example ex2: GAP term2 = 0 := ltac:(trivial).
-  Example ex3: GAP term3 = 0 := ltac:(trivial).
-  Example ex3a: GAP term3a = 0 := ltac:(trivial).
-  Example ex4: GAP term4 = 0 := ltac:(trivial).
-
+  Example ex1: level term1 = 0 := ltac:(trivial).
+  Example ex2: level term2 = 0 := ltac:(trivial).
+  Example ex3: level term3 = 0 := ltac:(trivial).
+  Example ex4: level term4 = 0 := ltac:(trivial).
+  Example ex5: level term5 = 1 := ltac:(trivial).
 End demo3.
