Tealeaves/Misc/NaturalNumbers.v
@@ -9,3 +9,56 @@ From Tealeaves Require Import
 #[global, program] Instance Monoid_Nat : @Monoid nat Monoid_op_plus Monoid_unit_zero.
 
 Solve Obligations with (intros; unfold transparent tcs; lia).
+
+(** * Natural numbers with maximum *)
+#[local] Instance Monoid_op_max : Monoid_op nat := max.
+
+#[local] Instance Monoid_unit_max : Monoid_unit nat := 0.
+
+#[local, program] Instance Monoid_Nat_max : @Monoid nat Monoid_op_max Monoid_unit_max.
+
+Solve Obligations with (intros; unfold transparent tcs; lia).
+
+#[global] Instance PreOrder_Nat_lt:
+  @PreOrder nat le.
+Proof.
+  constructor; cbv; lia.
+Qed.
+
+#[global] Instance PreOrderedMonoidLaws_Nat_plus:
+  @PreOrderedMonoidLaws nat le Monoid_op_plus Monoid_unit_zero.
+Proof.
+  constructor; unfold transparent tcs; lia.
+Qed.
+
+#[global] Instance PreOrderedMonoid_Nat_plus:
+  @PreOrderedMonoid nat le Monoid_op_plus Monoid_unit_zero.
+Proof.
+  constructor; typeclasses eauto.
+Qed.
+
+#[global] Instance PreOrderedMonoidPos_Nat_plus:
+  @PreOrderedMonoidPos nat le Monoid_op_plus Monoid_unit_zero.
+Proof.
+  constructor; try typeclasses eauto.
+  cbv. lia.
+Qed.
+
+#[global] Instance PreOrderedMonoidLaws_Nat_max:
+  @PreOrderedMonoidLaws nat le Monoid_op_max Monoid_unit_max.
+Proof.
+  constructor; unfold transparent tcs; lia.
+Qed.
+
+#[global] Instance PreOrderedMonoid_Nat_max:
+  @PreOrderedMonoid nat le Monoid_op_max Monoid_unit_max.
+Proof.
+  constructor; typeclasses eauto.
+Qed.
+
+#[global] Instance PreOrderedMonoidPos_Nat_max:
+  @PreOrderedMonoidPos nat le Monoid_op_max Monoid_unit_max.
+Proof.
+  constructor; try typeclasses eauto.
+  cbv. lia.
+Qed.
